code/ecdsa/Hacl.Impl.EC.Reduction.fst
@@ -1,0 +1,30 @@
+module Hacl.Impl.EC.Reduction
+
+open FStar.HyperStack.All
+open FStar.HyperStack
+module ST = FStar.HyperStack.ST
+
+open Lib.IntTypes
+open FStar.Math.Lemmas
+open FStar.Math.Lib
+open Lib.Buffer
+
+open Hacl.SolinasReduction.Lemmas
+open Spec.P256
+open Hacl.Impl.EC.LowLevel
+
+open Hacl.Impl.SolinasReduction.P384
+open Hacl.Impl.SolinasReduction.P256
+
+open Hacl.Spec.P256.Definition
+open FStar.Mul
+
+module BV = FStar.BitVector
+module Seq = FStar.Seq
+
+#reset-options "--fuel 0 --ifuel 0 --z3rlimit 50"
+
+let reduction #c i o =
+  match c with 
+    |P256 -> solinas_reduction_impl_p256 i o 
+    |P384 -> solinas_reduction_impl_p384 i o
