code/ecdsa/Hacl.Impl.SolinasReduction.P384.fsti
@@ -16,7 +16,7 @@ open Lib.Buffer
 open Spec.P256
 open Hacl.Spec.P256.Definition
 
-val solinasReduction384Impl: i: lbuffer uint64 (size 12) -> o: lbuffer uint64 (size 6) -> 
+val solinas_reduction_impl_p384: i: lbuffer uint64 (size 12) -> o: lbuffer uint64 (size 6) -> 
   Stack unit 
     (requires fun h -> live h i /\ live h o /\ disjoint i o)
     (ensures fun h0 _ h1 -> modifies (loc o) h0 h1 /\ wide_as_nat P384 h0 i % prime384 = as_nat P384 h1 o)
